Foundation.lean
@@ -143,6 +143,7 @@ import Foundation.Modal.Neighborhood.Logic.EMCN
 import Foundation.Modal.Neighborhood.Logic.EMT4
 import Foundation.Modal.Neighborhood.Logic.END
 import Foundation.Modal.Neighborhood.Logic.ET4
+import Foundation.Modal.Neighborhood.Logic.E5
 import Foundation.Modal.Neighborhood.Logic.Incomparability.ED_EP
 
 import Foundation.Modal.ModalCompanion.Int
