Foundation/Modal/Entailment/E.lean
@@ -1,0 +1,38 @@
+import Foundation.Modal.Entailment.DiaDuality
+
+namespace LO.Modal.Entailment
+
+open LO.Entailment LO.Entailment.FiniteContext
+
+variable {S F : Type*} [BasicModalLogicalConnective F] [Entailment F S]
+variable {𝓢 : S} [Entailment.E 𝓢] {n : ℕ} {φ ψ ξ χ: F}
+
+variable [DecidableEq F]
+
+def ELLNN! : 𝓢 ⊢! □φ ⭤ □(∼∼φ) := by apply re; exact dn;
+@[simp] lemma ELLNN : 𝓢 ⊢ □φ ⭤ □(∼∼φ) := ⟨ELLNN!⟩
+
+def ILLNN! : 𝓢 ⊢! □φ ➝ □(∼∼φ) := K_left ELLNN!
+@[simp] lemma ILLNN : 𝓢 ⊢ □φ ➝ □(∼∼φ) := ⟨ILLNN!⟩
+alias box_dni := ILLNN!
+alias box_dni! := ILLNN
+
+def ILNNL! : 𝓢 ⊢! □(∼∼φ) ➝ □φ := K_right ELLNN!
+@[simp] lemma ILNNL : 𝓢 ⊢ □(∼∼φ) ➝ □φ := ⟨ILNNL!⟩
+alias box_dne := ILNNL!
+alias box_dne! := ILNNL
+
+def box_dne' (h : 𝓢 ⊢! □(∼∼φ)): 𝓢 ⊢! □φ := box_dne ⨀ h
+@[grind →] lemma box_dne'! (h : 𝓢 ⊢ □(∼∼φ)): 𝓢 ⊢ □φ := ⟨box_dne' h.some⟩
+
+@[simp] lemma INMNL : 𝓢 ⊢ ∼◇(∼φ) ➝ □φ := by
+  apply CN!_of_CN!_left;
+  apply C!_trans ?_ INLNM;
+  apply contra!;
+  simp;
+
+@[simp] lemma INLMN :  𝓢 ⊢ ∼□φ ➝ ◇(∼φ) := by
+  apply CN!_of_CN!_left;
+  simp;
+
+end LO.Modal.Entailment
