Foundation/Modal/Neighborhood/AxiomB.lean
@@ -1,0 +1,106 @@
+import Foundation.Modal.Neighborhood.AxiomGeach
+import Foundation.Modal.Neighborhood.Supplementation
+
+
+namespace LO.Modal
+
+
+section
+
+variable {α : Type*} [DecidableEq α]
+variable {S} [Entailment (Formula α) S]
+variable {𝓢 : S} [Entailment.Cl 𝓢]
+
+abbrev Proofset (𝓢 : S) := Set (MaximalConsistentSet 𝓢)
+abbrev Nonproofset (𝓢 : S) := { P : Proofset 𝓢 // ∀ φ, P ≠ proofset 𝓢 φ }
+
+end
+
+
+namespace Neighborhood
+
+section
+
+open MaximalConsistentSet
+
+variable [Entailment (Formula ℕ) S]
+variable {𝓢 : S} [Entailment.Consistent 𝓢] [Entailment.E 𝓢]
+
+def Canonicity.box (𝓒 : Canonicity 𝓢) : Proofset 𝓢 → Proofset 𝓢 := λ X => { w | X ∈ 𝓒.𝒩 w }
+def Canonicity.dia (𝓒 : Canonicity 𝓢) : Proofset 𝓢 → Proofset 𝓢 := λ X => (𝓒.box Xᶜ)ᶜ
+
+abbrev relativeMinimalCanonicity (𝓢 : S) [Entailment.E 𝓢] (𝓧 : MaximalConsistentSet 𝓢 → Set (Proofset 𝓢)) (h𝓧 : ∀ A, ∀ X ∈ 𝓧 A, ∀ φ, X ≠ proofset 𝓢 φ) : Canonicity 𝓢 where
+  𝒩 A := (minimalCanonicity 𝓢 |>.𝒩 A) ∪ (𝓧 A);
+  def_𝒩 := by
+    intro X φ;
+    constructor;
+    . intro h;
+      left;
+      use φ;
+    . rintro (⟨ψ, hψ₁, hψ₂⟩ | h);
+      . have := proofset.eq_boxed_of_eq hψ₂;
+        grind;
+      . simpa using h𝓧 _ _ h φ;
+  V a := proofset 𝓢 (.atom a);
+  def_V := by simp;
+
+abbrev relativeMinimalCanonicity.of_box (𝓢 : S) [Entailment.E 𝓢]
+  (𝓑 : Proofset 𝓢 → Proofset 𝓢)
+  (h𝓑 : ∀ X, ∀ A ∈ 𝓑 X, ∀ φ, X ≠ proofset 𝓢 φ)
+  : Canonicity 𝓢 := relativeMinimalCanonicity 𝓢
+  (λ x => { X | x ∈ 𝓑 X })
+  (by grind)
+
+abbrev canonicity_for_EB (𝓢 : S) [Entailment.E 𝓢] : Canonicity 𝓢 := relativeMinimalCanonicity.of_box 𝓢 (λ X A => (∀ φ, X ≠ proofset 𝓢 φ) ∧ (minimalCanonicity 𝓢).dia ((minimalCanonicity 𝓢).box X) A) $ by
+  rintro X A ⟨_, _⟩;
+  assumption;
+
+instance [Entailment.HasAxiomB 𝓢] : (canonicity_for_EB 𝓢).toModel.IsSymmetric := by
+  constructor;
+  intro X Γ hΓ;
+  by_cases h : ∀ φ, X ≠ proofset 𝓢 φ;
+  . sorry;
+  . push_neg at h;
+    obtain ⟨φ, rfl⟩ := h;
+    simp only [Canonicity.dia_proofset, Canonicity.box_proofset] at hΓ ⊢;
+    apply proofset.imp_subset.mp (by simp) hΓ;
+
+def maximalCanonicity (𝓢 : S) [Entailment.E 𝓢] : Canonicity 𝓢 where
+  𝒩 A := (minimalCanonicity 𝓢 |>.𝒩 A) ∪ ({ X | ∀ φ, X ≠ proofset 𝓢 φ})
+  def_𝒩 := by
+    intro X φ;
+    constructor;
+    . intro h;
+      left;
+      use φ;
+    . rintro (⟨ψ, hψ₁, hψ₂⟩ | h);
+      . have := proofset.eq_boxed_of_eq hψ₂;
+        grind;
+      . grind;
+  V a := proofset 𝓢 (.atom a);
+  def_V := by simp;
+
+open LO.Entailment
+
+instance [Entailment.HasAxiomFive 𝓢] : (maximalCanonicity 𝓢).toModel.IsEuclidean := by
+  apply Frame.IsEuclidean.of_alt;
+  rintro A X hX;
+  obtain ⟨hX, ⟨φ, rfl⟩⟩ : X ∉ (minimalCanonicity 𝓢).𝒩 A ∧ ∃ x, X = proofset 𝓢 x := by simpa [Canonicity.toModel, maximalCanonicity] using hX;
+
+  suffices proofset 𝓢 (◇(∼φ)) = {b | proofset 𝓢 φ ∉ (maximalCanonicity 𝓢).toModel.𝒩 b} by
+    have H : proofset 𝓢 (◇(∼φ)) ∈ (maximalCanonicity 𝓢).𝒩 A := (maximalCanonicity 𝓢).def_𝒩 _ _ |>.mp
+      $ MaximalConsistentSet.mdp_provable (show 𝓢 ⊢ ∼□φ ➝ □◇(∼φ) by exact C!_trans (by simp) Entailment.axiomFive!)
+      $ MaximalConsistentSet.iff_mem_neg.mpr
+      $ by apply Canonicity.iff_box.not.mpr; simpa [Canonicity.toModel, maximalCanonicity];
+    rwa [this] at H;
+
+  ext _;
+  simp [←(maximalCanonicity 𝓢).dia_proofset, Canonicity.toModel];
+
+instance [Entailment.HasAxiomB 𝓢] : (maximalCanonicity 𝓢).toModel.IsSymmetric := by sorry;
+
+end
+
+end Neighborhood
+
+end LO.Modal
