Foundation/Modal/Neighborhood/AxiomGeach.lean
@@ -21,6 +21,13 @@ class IsReflexive (F : Frame) : Prop where
   refl : ∀ X : Set F, F.box X ⊆ X
 
 @[simp, grind] lemma refl [F.IsReflexive] : F.box X ⊆ X := IsReflexive.refl X
+@[simp, grind] lemma refl_dual [F.IsReflexive] : X ⊆ F.dia X := by
+  intro x;
+  contrapose!;
+  intro h;
+  have := F.refl (X := Xᶜ);
+  have := @this x;
+  simp_all [Frame.dia, Frame.box];
 
 instance [F.IsReflexive] : F.IsGeachConvergent ⟨0, 0, 1, 0⟩ := ⟨by simp⟩
 
@@ -57,8 +64,35 @@ lemma IsSymmetric.of_dual {F : Frame} (h : ∀ X : Set F, F.dia (F.box X) ⊆ X)
   have := @h Xᶜ w;
   simp_all;
 
+
 class IsEuclidean (F : Frame) : Prop where
   eucl : ∀ X : Set F, F.dia X ⊆ F.box (F.dia X)
+
+@[simp] lemma eucl [F.IsEuclidean] : F.dia X ⊆ F.box (F.dia X) := IsEuclidean.eucl X
+
+@[simp] lemma eucl_dual [F.IsEuclidean] : F.dia (F.box X) ⊆ F.box X := by
+  intro x;
+  contrapose!;
+  intro h;
+  have := F.eucl (X := Xᶜ);
+  have := @this x;
+  simp_all [Frame.dia, Frame.box];
+
+lemma IsEuclidean.of_dual {F : Frame} (h : ∀ X, F.dia (F.box X) ⊆ F.box X) : F.IsEuclidean := by
+  constructor;
+  intro X w hw;
+  have := @h Xᶜ w;
+  simp_all;
+
+lemma IsEuclidean.of_alt {F : Frame} (h : ∀ a X, X ∉ F.𝒩 a → { b | X ∉ F.𝒩 b } ∈ F.𝒩 a) : F.IsEuclidean := by
+  constructor;
+  intro X a ha;
+  have := h a;
+  simp_all [Frame.dia, Frame.box];
+  grind;
+
+instance [F.IsEuclidean] : F.IsGeachConvergent ⟨1, 1, 0, 1⟩ := ⟨by simp⟩
+instance [F.IsGeachConvergent ⟨1, 1, 0, 1⟩] : F.IsEuclidean := ⟨λ _ => F.gconv (g := ⟨1, 1, 0, 1⟩)⟩
 
 end Frame
 
@@ -75,9 +109,10 @@ lemma valid_axiomGeach_of_isGeachConvergent [F.IsGeachConvergent g] : F ⊧ Axio
   apply F.gconv;
 
 @[simp] lemma valid_axiomT_of_isReflexive [F.IsReflexive] : F ⊧ Axioms.T (.atom a) := valid_axiomGeach_of_isGeachConvergent (g := ⟨0, 0, 1, 0⟩)
-@[simp] lemma valid_axiomFour_of_isTransitive [F.IsTransitive] : F ⊧ Axioms.Four (.atom a) := valid_axiomGeach_of_isGeachConvergent (g := ⟨0, 2, 1, 0⟩)
 @[simp] lemma valid_axiomD_of_isSerial [F.IsSerial] : F ⊧ Axioms.D (.atom a) := valid_axiomGeach_of_isGeachConvergent (g := ⟨0, 0, 1, 1⟩)
 @[simp] lemma valid_axiomB_of_isSymmetric [F.IsSymmetric] : F ⊧ Axioms.B (.atom a) := valid_axiomGeach_of_isGeachConvergent (g := ⟨0, 1, 0, 1⟩)
+@[simp] lemma valid_axiomFour_of_isTransitive [F.IsTransitive] : F ⊧ Axioms.Four (.atom a) := valid_axiomGeach_of_isGeachConvergent (g := ⟨0, 2, 1, 0⟩)
+@[simp] lemma valid_axiomFive_of_isEuclidean [F.IsEuclidean] : F ⊧ Axioms.Five (.atom a) := valid_axiomGeach_of_isGeachConvergent (g := ⟨1, 1, 0, 1⟩)
 
 lemma isGeachConvergent_of_valid_axiomGeach (h : F ⊧ Axioms.Geach g (.atom a)) : F.IsGeachConvergent g := by
   constructor;
@@ -101,6 +136,10 @@ lemma isSerial_of_valid_axiomD (h : F ⊧ Axioms.D (.atom a)) : F.IsSerial := by
 
 lemma isSymmetric_of_valid_axiomB (h : F ⊧ Axioms.B (.atom a)) : F.IsSymmetric := by
   have := isGeachConvergent_of_valid_axiomGeach (g := ⟨0, 1, 0, 1⟩) h;
+  infer_instance;
+
+lemma isEuclidean_of_valid_axiomFive (h : F ⊧ Axioms.Five (.atom a)) : F.IsEuclidean := by
+  have := isGeachConvergent_of_valid_axiomGeach (g := ⟨1, 1, 0, 1⟩) h;
   infer_instance;
 
 end
@@ -134,71 +173,6 @@ instance [Entailment.HasAxiomD 𝓢] : (minimalCanonicity 𝓢).toModel.IsSerial
   obtain ⟨φ, rfl, _, hφ⟩ := minimalCanonicity.iff_mem_box_exists_fml.mp hΓ;
   simp only [Canonicity.dia_proofset];
   apply proofset.imp_subset.mp (by simp) hφ;
-
-/-
-instance [Entailment.HasAxiomGeach g 𝓢] : (minimalCanonicity 𝓢).IsGeachConvergent g := by
-  constructor;
-  intro X Γ hΓ;
-  obtain ⟨φ, rfl, hφ⟩ : ∃ φ, X = proofset 𝓢 φ ∧ Γ ∈ proofset 𝓢 (◇^[g.i](□^[g.m]φ)) := by
-    sorry;
-  simp only [minimalCanonicalFrame.multidia_proofset, minimalCanonicalFrame.multibox_proofset] at hΓ ⊢;
-  apply proofset.imp_subset.mp (by simp) hφ;
-
-open Classical in
-instance [Entailment.HasAxiomB 𝓢] : (minimalCanonicity 𝓢).IsSymmetric := by
-  constructor;
-  intro X Γ hΓ;
-  dsimp [minimalCanonicalFrame, Frame.mk_ℬ, Frame.dia, Frame.box];
-  generalize eY : (if h : ∃ φ, Xᶜ = proofset 𝓢 φ then proofset 𝓢 (□h.choose) else ∅) = Y;
-  generalize eZ : (if h : ∃ φ, Yᶜ = proofset 𝓢 φ then proofset 𝓢 (□h.choose) else ∅) = Z;
-  split_ifs at eY eZ with hY hZ hZ;
-  . obtain ⟨φ, hY₁⟩ := hY;
-    obtain ⟨ψ, hZ₁⟩ := hZ;
-    sorry;
-  . subst eY eZ;
-    push_neg at hZ;
-    simpa using hZ (∼□hY.choose);
-  . subst eY eZ;
-    push_neg at hY;
-    have := hY (∼□hZ.choose);
-
-    sorry;
-  . subst eY eZ;
-    push_neg at hZ;
-    simpa using hZ ⊤;
-
-open Classical in
-instance [Entailment.HasAxiomFive 𝓢] : (minimalCanonicity 𝓢).IsEuclidean := by
-  constructor;
-  intro X Γ hΓ;
-  dsimp [minimalCanonicalFrame, Frame.mk_ℬ, Frame.dia, Frame.box];
-  generalize eh : (if h : ∃ φ, Xᶜ = proofset 𝓢 φ then proofset 𝓢 (□h.choose) else ∅)ᶜ = Y;
-  split_ifs at eh with hif₁;
-  . split_ifs with hif₂;
-    . rcases (minimalCanonicalFrame.iff_exists_dia.mp hΓ) hif₂.choose with (a | a | a)
-      . sorry;
-      . sorry;
-      . sorry;
-    . exfalso;
-      push_neg at hif₂;
-      apply hif₂ (∼□(hif₁.choose));
-      grind;
-  . subst eh;
-    split_ifs with hif₂;
-    . push_neg at hif₁;
-      obtain ⟨φ, a₂⟩ := hif₂;
-      have := hif₂.choose_spec;
-      generalize hif₂.choose = ψ at this hif₁ ⊢;
-      rcases (minimalCanonicalFrame.iff_exists_dia.mp hΓ) ψ with (a | a | a)
-      . rw [←this] at a;
-        simp at a;
-        sorry;
-      . have := hif₁ ψ;
-        sorry;
-      . sorry;
-    . push_neg at hif₂;
-      simpa using hif₂ ⊤;
--/
 
 end
 
