Foundation/Modal/Neighborhood/Logic/E5.lean
@@ -1,0 +1,49 @@
+import Foundation.Modal.Neighborhood.AxiomGeach
+import Foundation.Modal.Neighborhood.AxiomM
+import Foundation.Modal.Neighborhood.AxiomC
+import Foundation.Modal.Neighborhood.AxiomB
+import Foundation.Modal.Neighborhood.Logic.E
+import Foundation.Modal.Neighborhood.Filtration
+
+namespace LO.Modal
+
+open Neighborhood
+open Hilbert.Neighborhood
+open Formula.Neighborhood
+
+namespace Neighborhood
+
+
+@[reducible] protected alias Frame.IsE5 := Frame.IsEuclidean
+protected class Frame.IsFiniteE5 (F : Frame) extends F.IsE5, F.IsFinite
+
+protected abbrev FrameClass.E5 : FrameClass := { F | F.IsE5 }
+protected abbrev FrameClass.finite_E5 : FrameClass := { F | F.IsFiniteE5 }
+
+instance : Frame.simple_blackhole.IsEuclidean := by
+  constructor;
+  intro X x hx;
+  simp_all [(show X ≠ ∅ by grind), Frame.box];
+
+end Neighborhood
+
+namespace E5
+
+instance : Sound Modal.E5 FrameClass.E5 := instSound_of_validates_axioms $ by
+  simp only [Semantics.RealizeSet.singleton_iff];
+  intro F hF;
+  replace hF := Set.mem_setOf_eq.mp hF;
+  apply valid_axiomFive_of_isEuclidean;
+
+instance : Entailment.Consistent Modal.E5 := consistent_of_sound_frameclass FrameClass.E5 $ by
+  use Frame.simple_blackhole;
+  apply Set.mem_setOf_eq.mpr;
+  infer_instance
+
+instance : Complete Modal.E5 FrameClass.E5 := (maximalCanonicity _).completeness $ by
+  apply Set.mem_setOf_eq.mpr;
+  infer_instance;
+
+end E5
+
+end LO.Modal
