Foundation/Modal/Neighborhood/Logic/EM.lean
@@ -68,7 +68,7 @@ instance : Entailment.Consistent Modal.EM := consistent_of_sound_frameclass Fram
   simp only [Set.mem_setOf_eq];
   infer_instance;
 
-instance : Complete Modal.EM FrameClass.EM := (maximalCanonicity Modal.EM).completeness $ by
+instance : Complete Modal.EM FrameClass.EM := (supplementedMinimalCanonicity Modal.EM).completeness $ by
   apply Set.mem_setOf_eq.mpr;
   infer_instance;
 
