Foundation/Modal/Neighborhood/Logic/EMCN.lean
@@ -29,7 +29,7 @@ instance : Entailment.Consistent Modal.EMCN := consistent_of_sound_frameclass Fr
   simp only [Set.mem_setOf_eq];
   constructor;
 
-instance : Complete Modal.EMCN FrameClass.EMCN := (maximalCanonicity Modal.EMCN).completeness $ by
+instance : Complete Modal.EMCN FrameClass.EMCN := (supplementedMinimalCanonicity Modal.EMCN).completeness $ by
   apply Set.mem_setOf_eq.mpr;
   constructor;
 
