Foundation/Modal/Neighborhood/Logic/ET5.lean
@@ -1,0 +1,68 @@
+import Foundation.Modal.Neighborhood.AxiomGeach
+import Foundation.Modal.Neighborhood.AxiomN
+import Foundation.Modal.Neighborhood.Logic.ED
+import Foundation.Modal.Neighborhood.Logic.ET4
+
+
+namespace LO.Modal
+
+open Neighborhood
+open Hilbert.Neighborhood
+open Formula.Neighborhood
+
+namespace Neighborhood
+
+protected class Frame.IsET5 (F : Frame) extends F.IsReflexive, F.IsEuclidean
+protected abbrev FrameClass.ET5 : FrameClass := { F | F.IsET5 }
+
+variable {F : Frame}
+
+instance [F.IsReflexive] : F.NotContainsEmpty where
+  not_contains_empty := by apply F.refl;
+
+instance [F.IsReflexive] [F.IsEuclidean] : F.ContainsUnit where
+  contains_unit := by
+    ext x;
+    suffices x ∈ F.box Set.univ by simpa;
+    have H₁ : x ∈ (F.box $ F.dia Set.univ) → x ∈ (F.box $ Set.univ) := by simp [show F.dia Set.univ = Set.univ by ext; simp]
+    apply H₁;
+    apply F.eucl;
+    simp;
+
+instance : Frame.simple_blackhole.IsET5 where
+  eucl := by
+    intro X x hx;
+    simp_all [Frame.simple_blackhole, Frame.box];
+
+end Neighborhood
+
+
+namespace ET5
+
+instance : Sound Modal.ET5 FrameClass.ET5 := instSound_of_validates_axioms $ by
+  constructor;
+  rintro _ (rfl | rfl) F (rfl | rfl) <;> simp;
+
+instance : Entailment.Consistent Modal.ET5 := consistent_of_sound_frameclass FrameClass.ET5 $ by
+  use Frame.simple_blackhole;
+  simp only [Set.mem_setOf_eq];
+  infer_instance;
+
+instance : Complete Modal.ET5 FrameClass.ET5 := (minimalCanonicity Modal.ET5).completeness $ by sorry;
+
+end ET5
+
+
+instance : Modal.END4 ⪱ Modal.ET5 := by
+  constructor;
+  . apply Hilbert.WithRE.weakerThan_of_provable_axioms;
+    rintro φ (rfl | rfl | rfl);
+    . apply Complete.complete (𝓜 := FrameClass.ET5)
+      intro F hF;
+      replace hF := Set.mem_setOf_eq.mp hF;
+      apply valid_axiomN_of_ContainsUnit
+    . sorry;
+    . sorry;
+  . sorry;
+
+end LO.Modal
